Partial progress on proving enumerator semantics

src/Enumerators/Enumerators.dfy
@@ -13,6 +13,10 @@ module Enumerators {
 
   trait {:termination false} Enumerator<T> extends Validatable {
     
+    // The Valid() predicate from the Validatable trait ends up
+    // becoming the "enumeration invariant", which in turn becomes
+    // the loop invariant in a while loop that uses an enumerator.
+
     ghost var enumerated: seq<T>
 
     // Any enumerator that produces one value at a time
@@ -22,6 +26,12 @@ module Enumerators {
     // values have been produced.
     // Dafny doesn't let you pass around an underspecified value though,
     // so we don't define a "to be enumerated" field or function.
+
+    predicate method HasNext() 
+      reads Repr
+      requires Valid()
+      decreases Repr, 0
+      ensures Decreases() == 0 ==> !HasNext()
 
     method Next() returns (element: T)
       requires Valid()
@@ -39,16 +49,10 @@ module Enumerators {
       reads Repr
       decreases Repr
       requires Valid()
-
-    predicate method HasNext() 
-      reads Repr
-      requires Valid()
-      decreases Repr, 0
-      ensures Decreases() == 0 ==> !HasNext()
   }
 
   // TODO: Common EagerEnumerator<T> that wraps a Enumerator<Option<T>>
-  // for cases like Filter or IteratorAdaptor that can't calculate Done() 
+  // for cases like Filter or IteratorAdaptor that can't calculate HasNext() 
   // ahead of time?
 
   class SeqEnumerator<T> extends Enumerator<T> {
@@ -59,6 +63,8 @@ module Enumerators {
     constructor(s: seq<T>) 
       ensures Valid()
       ensures fresh(Repr - {this})
+      ensures enumerated == []
+      ensures elements == s
     {
       elements := s;
       index := 0;
@@ -117,6 +123,8 @@ module Enumerators {
     constructor(s: set<T>) 
       ensures Valid() 
       ensures fresh(Repr)
+      ensures enumerated == []
+      ensures original == s
     {
       this.original := s;
       this.remaining := s;
@@ -127,9 +135,10 @@ module Enumerators {
 
     predicate Valid() 
       reads this, Repr 
-      ensures Valid() ==> this in Repr 
+      ensures Valid() ==> this in Repr
     {
       && this in Repr
+      && multiset(enumerated) + multiset(remaining) == multiset(original)
     }
 
     predicate method HasNext()
@@ -165,17 +174,23 @@ module Enumerators {
     }
   }
 
-  class MapEnumerator<T, R> extends Enumerator<R> {
+  class MappingEnumerator<T, R> extends Enumerator<R> {
     const wrapped: Enumerator<T>
     const f: T -> R
 
     constructor(f: T -> R, wrapped: Enumerator<T>) 
       requires wrapped.Valid()
+      requires wrapped.enumerated == []
       ensures Valid() 
+      ensures fresh(Repr - wrapped.Repr)
+      ensures enumerated == []
+      ensures this.wrapped == wrapped
+      ensures this.f == f
     {
       this.wrapped := wrapped;
       this.f := f;
       Repr := {this} + wrapped.Repr;
+      enumerated := [];
     }
 
     predicate Valid() 
@@ -185,6 +200,7 @@ module Enumerators {
     {
       && this in Repr
       && ValidComponent(wrapped)
+      && enumerated == Seq.Map(f, wrapped.enumerated)
     }
 
     predicate method HasNext()
@@ -219,7 +235,7 @@ module Enumerators {
     }
   }
 
-  class ConcatEnumerator<T(0)> extends Enumerator<T> {
+  class ConcatEnumerator<T> extends Enumerator<T> {
 
     // TODO: Unset once each is Done() to allow garbage collection?
     const first: Enumerator<T>
@@ -231,6 +247,8 @@ module Enumerators {
       requires first.Repr !! second.Repr
       ensures Valid() 
       ensures fresh(Repr - first.Repr - second.Repr) 
+      ensures this.first == first
+      ensures this.second == second
     {
       this.first := first;
       this.second := second;
@@ -244,7 +262,8 @@ module Enumerators {
       && ValidComponent(first)
       && ValidComponent(second)
       && first.Repr !! second.Repr
-      // && enumerated == first.enumerated + second.enumerated
+      // && (first.HasNext() ==> second.enumerated == [])
+      && enumerated == first.enumerated + second.enumerated
     }
 
     predicate method HasNext()
@@ -290,18 +309,17 @@ module Enumerators {
     const filter: T -> bool
     var next: Option<T>
 
-    ghost var decr: nat
-
     constructor(wrapped: Enumerator<T>, filter: T -> bool) 
       requires wrapped.Valid()
+      requires wrapped.enumerated == []
       modifies wrapped.Repr
-      ensures Valid() 
+      ensures Valid()
     {
       this.wrapped := wrapped;
       this.filter := filter;
       this.next := None;
       Repr := {this} + wrapped.Repr;
-      decr := wrapped.Decreases();
+      enumerated := [];
       new;
       FindNext();
     }
@@ -309,6 +327,7 @@ module Enumerators {
     predicate Valid() reads this, Repr ensures Valid() ==> this in Repr {
       && this in Repr
       && ValidComponent(wrapped)
+      // && (if next.Some? then enumerated + [next.value] else enumerated) == Seq.Filter(filter, wrapped.enumerated)
     }
 
     predicate method HasNext()
@@ -377,31 +396,52 @@ module Enumerators {
     }
   }
 
-  // method Max(s: set<int>) returns (max: int)
-  //   requires |s| > 0
-  //   ensures max in s
-  //   ensures forall x | x in s :: max >= x
-  // {
-  //   var first: int :| first in s;
-  //   max := first;
-  //   var sEnum: SetEnumerator<int> := new SetEnumerator(s - {max});
-  //   assert fresh(sEnum.Repr);
-  //   label start:
-  //   var more := true;
-  //   while (!sEnum.Done()) 
-  //     invariant sEnum.Valid()
-  //     invariant fresh(sEnum.Repr)
-  //     invariant max == Seq.Max([first] + sEnum.enumerated)
-  //     decreases more, sEnum.Decreases()
-  //   {
-  //     var more := sEnum.MoveNext();
-  //     if !more { break; }
+  method CollectToSeq<T>(e: Enumerator<T>) returns (s: seq<T>)
+    requires e.Valid()
+    // TODO: Might remove this
+    requires e.enumerated == []
+    modifies e.Repr
+    ensures e.Valid()
+    ensures !e.HasNext()
+    ensures s == e.enumerated
+  {
+    s := [];
+    while (e.HasNext())
+      invariant e.Valid() && e.Repr <= old(e.Repr)
+      decreases e.Decreases()
 
-  //     if sEnum.Current() > max {
-  //       max := sEnum.Current();
-  //     }
-  //   }
-  // }
+      invariant s == e.enumerated
+    {
+      var element := e.Next();
+      s := s + [element];
+    }
+  }
+
+  method Max(s: set<int>) returns (max: int)
+    requires |s| > 0
+    ensures max in s
+    ensures forall x | x in s :: max >= x
+  {
+    var first: int :| first in s;
+    max := first;
+    var rest := s - {max};
+
+    var sEnum: SetEnumerator<int> := new SetEnumerator(rest);
+    while (sEnum.HasNext()) 
+      invariant sEnum.Valid()
+      invariant fresh(sEnum.Repr)
+      invariant max == Seq.Max([first] + sEnum.enumerated)
+      decreases sEnum.Decreases()
+    {
+      var element := sEnum.Next();
+
+      if max < element {
+        max := element;
+      }
+    }
+    assert max == Seq.Max([first] + sEnum.enumerated);
+    assert multiset(sEnum.enumerated) == multiset(rest);
+  }
 
   method Example1() {
     var numbers := [1, 2, 3, 4, 5];
@@ -452,7 +492,28 @@ module Enumerators {
     print "\n";
   }
 
-  // TODO: Explicit example of working with lazy iterators, more emphasis on `Done` being a pure function
+  method MappingExample() {
+    var first := [1, 2, 3, 4, 5];
+    var e1 := new SeqEnumerator(first);
+    var e := new MappingEnumerator(x => x + 2, e1);
+   
+    var result: seq<int> := [];
+    while (e.HasNext()) 
+      invariant e.Valid() && fresh(e.Repr)
+      decreases e.Decreases()
+    {
+      var element := e.Next();
+
+      result := result + [element];
+    }
+    assert e.enumerated == Seq.Map(x => x + 2, first);
+  }
+
+  // TODO: Explicit example of working with lazy iterators, more emphasis on `HasNext` being a pure function
   // TODO: Need to give background on Validatable, the fact that Valid() is the loop invariant
   // TODO: Mention `enumerated` ghost variable, proving semantics based on that
+  // TODO: Are ghost enumerators a thing? :)
+  // TODO: Most enumerator constructors should ensure enumerated == [] and other things
+  //       Important to have end to end examples to ensure correctness invariants are actually usable!
+  // TODO: Framing invariant is a pain in the butt, seems to need a label to be generic
 }
