examples/Enumerators/Enumerators.dfy
@@ -1,0 +1,53 @@
+include "../../src/Enumerators/Enumerators.dfy"
+
+module Demo {
+
+  import opened Enumerators
+
+  method AddTwoToEach(s: seq<nat>) returns (result: seq<nat>)
+    ensures forall x | x in result :: x >= 2
+  {
+    result := Seq.Map(x => x + 2, s);
+  }
+
+  method RoundTrip(s: seq<nat>) returns (result: seq<nat>)
+    ensures result == s
+  {
+    var e: SeqEnumerator := new SeqEnumerator(s);
+    result := CollectToSeq(e);
+  }
+
+  method AddTwoToEachEnumeratorVersion(s: seq<nat>) returns (result: seq<nat>)
+    ensures result == Seq.Map(x => x + 2, s)
+  {
+    var e := new SeqEnumerator(s);
+    var mapped := new MappingEnumerator(x => x + 2, e);
+    result := CollectToSeq(mapped);
+  }
+
+  method SetToSeq<T>(s: set<T>) returns (result: seq<T>)
+    ensures multiset(result) == multiset(s)
+  {
+    var e := new SetEnumerator(s);
+    result := CollectToSeq(e);
+  }
+
+  method Filter<T>(s: seq<T>, p: T -> bool) returns (result: seq<T>)
+    ensures result == Seq.Filter(p, s)
+  {
+    var e := new SeqEnumerator(s);
+    var filtered := new Filter<T>(e, p);
+    result := CollectToSeq(e);
+  }
+
+  method Concatenate<T>(first: seq<T>, second: seq<T>) returns (result: seq<T>)
+    ensures result == first + second
+  {
+    var e1: Enumerator<T> := new SeqEnumerator(first);
+    var e2 := new SeqEnumerator(second);
+    var concatenated: ConcatEnumerator := new ConcatEnumerator(e1, e2);
+    result := CollectToSeq(concatenated);
+    assert concatenated.Valid();
+  }
+
+}
